two parameters in the syntax to improve sharing/reification/notations (temporarily breaks ability to provide terms)

syntax.v
@@ -8,129 +8,140 @@ Unset Strict Implicit.
 Unset Printing Implicit Defensive.
 
 (** sorts of expressions we know how to approximate 
-    - real numbers
-    - functions on closed real intervals
-    - (conjunctions/disjunctions) comparison of reals
-    - (conjunctions/disjunctions) comparison of models
+    - [term ZER REAL]: real numbers (R)
+    - [term ONE REAL]: functions on closed real intervals (R->R), seen as reals with one real parameter
+    - [term ZER PROP]: (conjunctions/disjunctions) comparison of reals (Prop)
+    - [term ONE PROP]: (conjunctions/disjunctions) comparison of functions, seen as propositions with one real parameter (R -> Prop)
  *)
-Variant sort := REAL | FUN | BOOL | PRED.
+Variant csort := REAL | PROP.
+Variant dsort := ZER | ONE.
 
 (** syntax for the expressions we know how to approximate 
     we use parameterised higher order abstract syntax (PHOAS) in order to have a let..in construct and be able to share subexpressions
-    [@term X S] intuitively contains terms of sort [S] with variables in [X]
+    [@term X S T] intuitively contains terms of sort [S,T] with variables in [X]
 *)
-Inductive term {X: sort -> Type}: sort -> Type :=
+Inductive term {X: dsort -> csort -> Type}: dsort -> csort -> Type :=
 (* real expressions *)
-| e_add: term REAL -> term REAL -> term REAL
-| e_sub: term REAL -> term REAL -> term REAL
-| e_mul: term REAL -> term REAL -> term REAL
-| e_fromZ: Z -> term REAL
-| e_fromQ: Q -> term REAL
-| e_zer: term REAL
-| e_one: term REAL
-| e_pi: term REAL
-| e_div: term REAL -> term REAL -> term REAL
-| e_sqrt: term REAL -> term REAL
-| e_cos: term REAL -> term REAL
-| e_sin: term REAL -> term REAL
-| e_abs: term REAL -> term REAL
-| e_eval: term FUN -> term REAL -> term REAL
-| e_integrate: term FUN -> term REAL -> term REAL -> term REAL
-(* functional expressions *)
-| f_add: term FUN -> term FUN -> term FUN
-| f_sub: term FUN -> term FUN -> term FUN
-| f_mul: term FUN -> term FUN -> term FUN
-| f_div: term FUN -> term FUN -> term FUN
-| f_sqrt: term FUN -> term FUN
-| f_id: term FUN
-| f_cos: term FUN
-| f_sin: term FUN
-| f_cst: term REAL -> term FUN
-| f_trunc: nat -> term FUN -> term FUN         (* the identity, simply truncates the model *)
+| t_add: forall {D}, term D REAL -> term D REAL -> term D REAL
+| t_sub: forall {D}, term D REAL -> term D REAL -> term D REAL
+| t_mul: forall {D}, term D REAL -> term D REAL -> term D REAL
+| t_mul': forall {D}, nat -> term D REAL -> term D REAL -> term D REAL
+| t_div: forall {D}, term D REAL -> term D REAL -> term D REAL
+| t_sqrt: forall {D}, term D REAL -> term D REAL
+| t_cos: forall {D}, term D REAL -> term D REAL
+| t_sin: forall {D}, term D REAL -> term D REAL
+| t_abs: forall {D}, term D REAL -> term D REAL
+| t_fromZ: forall {D}, Z -> term D REAL
+| t_fromQ: forall {D}, Q -> term D REAL
+| t_zer: forall {D}, term D REAL
+| t_one: forall {D}, term D REAL
+| t_pi: forall {D}, term D REAL
+| t_id: term ONE REAL
+| t_app: term ONE REAL -> term ZER REAL -> term ZER REAL (* TOTHINK: also on PROP? *)
+| t_integrate: term ONE REAL -> term ZER REAL -> term ZER REAL -> term ZER REAL
+| t_trunc: nat -> term ONE REAL -> term ONE REAL         (* the identity, simply truncates the model *)
 (* boolean expressions *)
-(* TODO: true, false *)
-| b_le: term REAL -> term REAL -> term BOOL
-| b_ge: term REAL -> term REAL -> term BOOL
-| b_lt: term REAL -> term REAL -> term BOOL
-| b_ne: term REAL -> term REAL -> term BOOL
-    (* need b_ge and not b_gt because Rgt unfolds to Rlt while Rge does not unfold to Rle *)
-| b_disj: term BOOL -> term BOOL -> term BOOL
-| b_conj: term BOOL -> term BOOL -> term BOOL
-| b_forall_models: term REAL -> term REAL -> term PRED -> term BOOL
-| b_forall_bisect: term REAL -> term REAL -> (X REAL -> term BOOL) -> term BOOL
-(* univariate predicates *)
-(* TODO: c_le, c_ge *)
-(* TODO: true, false *)
-| c_lt: term FUN -> term FUN -> term PRED
-| c_ne: term FUN -> term FUN -> term PRED
-| c_disj: term PRED -> term PRED -> term PRED
-| c_conj: term PRED -> term PRED -> term PRED
-| c_cst: term BOOL -> term PRED
-| c_forall_bisect: term REAL -> term REAL -> (X REAL -> term PRED) -> term PRED
+| t_le: forall {D}, term D REAL -> term D REAL -> term D PROP
+| t_ge: forall {D}, term D REAL -> term D REAL -> term D PROP
+| t_lt: forall {D}, term D REAL -> term D REAL -> term D PROP
+| t_ne: forall {D}, term D REAL -> term D REAL -> term D PROP
+    (* don't need b_gt because Rgt unfolds to Rlt (while Rge does not unfold to Rle) *)
+| t_disj: forall {D}, term D PROP -> term D PROP -> term D PROP
+| t_conj: forall {D}, term D PROP -> term D PROP -> term D PROP
+| t_true: forall {D}, term D PROP
+| t_false: forall {D}, term D PROP
+| t_forall_models: term ZER REAL -> term ZER REAL -> term ONE PROP -> term ZER PROP
+| t_forall_bisect: forall {D}, term D REAL -> term D REAL -> (X ZER REAL -> term D PROP) -> term D PROP
+(* constant expressions not using their parameter *)
+| t_cst: forall {C}, term ZER C -> term ONE C
 (* setting the parameters in a subexpression *)
-| t_set {S}: prm -> term S -> term S
+| t_set {D C}: prm -> term D C -> term D C
 (* let..in and variable *)
-| t_var: forall {S}, X S -> term S
-| t_let: forall {S T}, term S -> (X S -> term T) -> term T.
-Definition let' {X S T}: @term X S -> (term S -> term T) -> term T :=
+| t_var: forall {D C}, X D C -> term D C
+| t_let: forall {D C F E}, term D C -> (X D C -> term F E) -> term F E.
+Definition t_let' {X D C F E}: @term X D C -> (term D C -> term F E) -> term F E :=
   fun a k => t_let a (fun x => k (t_var x)). 
-Definition f_trunc' {X} d u: @term X FUN := match d with None => u | Some d => f_trunc d u end.
+Definition t_forall_bisect' {X D}: term D REAL -> term D REAL -> (term ZER REAL -> term D PROP) -> @term X D PROP :=
+  fun a b k => t_forall_bisect a b (fun x => k (t_var x)). 
+Definition t_trunc' {X} d u: @term X ONE REAL := match d with None => u | Some d => t_trunc d u end.
 
 (** closed terms: they act polymorphically in X *)
-Definition Term S := forall X, @term X S.
-(** (terms of sort T with a single variable of sort S would be represented by type 
-    [forall X, X S -> @term X T]) *)
+Definition Term D C := forall X, @term X D C.
+(** (terms of sort D,C with a single variable of sort F,E would be represented by type 
+    [forall X, X F E -> @term X D C]) *)
+
+(** notations for terms, via canonical structures *)
+Canonical Structure t_Ops0 X D: Ops0 := {|
+  car := @term X D REAL;
+  add := t_add;
+  sub := t_sub;
+  mul := t_mul;
+  mul' := t_mul';
+  zer := t_zer;
+  one := t_one;
+  mulZ z := t_mul (t_fromZ z);
+  divZ z := t_div^~ (t_fromZ z);
+|}.
+Canonical Structure t_Ops1 X D: Ops1 := {|
+  ops0 := t_Ops0 X D;
+  fromZ := t_fromZ;
+  div := t_div;
+  sqrt := t_sqrt;
+  cos := t_cos;
+  sin := t_sin;
+  abs := t_abs;
+  pi := t_pi;
+|}.
 
 
 (** ** real number semantics of expressions  *)
-Definition rval S: Type := match S with REAL => R | FUN => (R -> R) | BOOL => Prop | PRED => R -> Prop end.
-Fixpoint sem S (t: @term rval S): rval S :=
-  match t in term S return rval S with
-  | e_add e f => sem e + sem f
-  | e_sub e f => sem e - sem f
-  | e_mul e f => sem e * sem f
-  | e_div e f => sem e / sem f
-  | e_sqrt e => sqrt (sem e)
-  | e_cos e => cos (sem e)
-  | e_sin e => sin (sem e)
-  | e_abs e => abs (sem e)
-  | e_fromQ q => Q2R q
-  | e_fromZ z => fromZ z
-  | e_zer => 0
-  | e_one => 1
-  | e_pi => pi
-  | e_eval f x => sem f (sem x)
-  | e_integrate f a b => RInt (sem f) (sem a) (sem b)
-  | f_add e f => (fun x => sem e x + sem f x)
-  | f_sub e f => (fun x => sem e x - sem f x)
-  | f_mul e f => (fun x => sem e x * sem f x)
-  | f_div e f => (fun x => sem e x / sem f x)
-  | f_sqrt e => (fun x => sqrt (sem e x))
-  | f_id => id
-  | f_cos => cos
-  | f_sin => sin
-  | f_cst e => (fun _ => sem e)
-  | f_trunc _ f => sem f
-  | b_le e f => sem e <= sem f
-  | b_ge e f => sem e >= sem f
-  | b_lt e f => sem e < sem f
-  | b_ne e f => sem e <> sem f
-  | b_disj b c => sem b \/ sem c
-  | b_conj b c => sem b /\ sem c
-  | b_forall_models a b k => forall x: R, sem a <= x <= sem b -> sem k x
-  | b_forall_bisect a b k => forall x: R, sem a <= x <= sem b -> sem (k x)
-  | c_lt f g => fun x => sem f x < sem g x
-  | c_ne f g => fun x => sem f x <> sem g x
-  | c_disj b c => fun x => sem b x \/ sem c x
-  | c_conj b c => fun x => sem b x /\ sem c x
-  | c_cst b => fun x => sem b
-  | c_forall_bisect a b k => fun x => forall y: R, sem a <= y <= sem b -> sem (k y) x
-  | t_set _ _ x => sem x
-  | t_var _ x => x
-  | t_let _ _ x k => sem (k (sem x))
+Definition rval D C: Type :=
+  match D,C with ZER,REAL => R | ONE,REAL => (R -> R) | ZER,PROP => Prop | ONE,PROP => R -> Prop end.
+Fixpoint sem D C (t: @term rval D C): rval D C :=
+  match t in term D C return rval D C with
+  | t_add (ZER|ONE) e f => sem e + sem f
+  | t_sub (ZER|ONE) e f => sem e - sem f
+  | t_mul (ZER|ONE) e f => sem e * sem f
+  | t_mul' (ZER|ONE) d e f => sem e *[d] sem f
+  | t_div (ZER|ONE) e f => sem e / sem f
+  | t_sqrt (ZER|ONE) e => sqrt (sem e)
+  | t_cos (ZER|ONE) e => cos (sem e)
+  | t_sin (ZER|ONE) e => sin (sem e)
+  | t_abs (ZER|ONE) e => abs (sem e)
+  | t_fromQ (ZER|ONE) q => fromQ q
+  | t_fromZ (ZER|ONE) z => fromZ z
+  | t_zer (ZER|ONE) => 0
+  | t_one (ZER|ONE) => 1
+  | t_pi (ZER|ONE) => pi
+  | t_id => fun x => x
+  | t_app f x => sem f (sem x)
+  | t_integrate f a b => RInt (sem f) (sem a) (sem b)
+  | t_cst (REAL|PROP) e => (fun _ => sem e)
+  | t_trunc _ f => sem f
+  | t_le ZER e f => sem e <= sem f
+  | t_ge ZER e f => sem e >= sem f
+  | t_lt ZER e f => sem e < sem f
+  | t_ne ZER e f => sem e <> sem f
+  | t_disj ZER b c => sem b \/ sem c
+  | t_conj ZER b c => sem b /\ sem c
+  | t_true ZER => True
+  | t_false ZER => False
+  | t_forall_bisect ZER a b k => forall x: R, sem a <= x <= sem b -> sem (k x)
+  | t_forall_models a b k => forall x: R, sem a <= x <= sem b -> sem k x
+  | t_le ONE e f => fun x => sem e x <= sem f x
+  | t_ge ONE e f => fun x => sem e x >= sem f x
+  | t_lt ONE e f => fun x => sem e x < sem f x
+  | t_ne ONE e f => fun x => sem e x <> sem f x
+  | t_disj ONE b c => fun x => sem b x \/ sem c x
+  | t_conj ONE b c => fun x => sem b x /\ sem c x
+  | t_true ONE => fun _ => True
+  | t_false ONE => fun _ => False
+  | t_forall_bisect ONE a b k => fun y => forall x: R, sem a y <= x <= sem b y -> sem (k x) y
+  | t_set _ _ _ x => sem x
+  | t_var _ _ x => x
+  | t_let _ _ _ _ x k => sem (k (sem x))
   end.
-Definition sem' S (u: Term S): rval S := sem (u rval).
-
+Definition sem' D C (u: Term D C): rval D C := sem (u rval).
 
 
 (** ** reification *)
@@ -144,140 +155,112 @@ Arguments f_unr [_ _] _ _ _ /.
 Lemma VAR: R. exact R0. Qed.
 Ltac reduce e :=
   eval cbn beta iota delta
-       [ROps0 ROps1 f_Ops0 car ops0 zer one add sub mul mul' div sqrt cos sin abs pi f_bin f_unr fromZ]
+       [ROps0 ROps1 f_Ops0 f_Ops1 car ops0 zer one add sub mul mul' div sqrt cos sin abs pi f_bin f_unr fromZ fromQ]
   in e.
-Ltac ereify e :=
-  lazymatch e
-  with
+
+Ltac reify e :=
+  lazymatch e with
   | sem' (fun X => ?e) => e
-  | R0 => uconstr:(e_zer)
-  | R1 => uconstr:(e_one)
-  | Rplus ?e ?f => let e:=ereify e in let f:=ereify f in uconstr:(e_add e f)
-  | Rminus ?e ?f => let e:=ereify e in let f:=ereify f in uconstr:(e_sub e f)
-  | Rmult ?e ?f => let e:=ereify e in let f:=ereify f in uconstr:(e_mul e f)
-  | Rdiv ?e ?f => let e:=ereify e in let f:=ereify f in uconstr:(e_div e f)
-  | R_sqrt.sqrt ?e => let e:=ereify e in uconstr:(e_sqrt e)
-  | Rtrigo_def.cos ?e => let e:=ereify e in uconstr:(e_cos e)
-  | Rtrigo_def.sin ?e => let e:=ereify e in uconstr:(e_sin e)
-  | Rabs ?e => let e:=ereify e in uconstr:(e_abs e)
-  | set ?p ?e => let e:=ereify e in uconstr:(t_set p e)
-  | Q2R ?q => uconstr:(e_fromQ q)
-  | IZR ?z => uconstr:(e_fromZ z)
-  | Rtrigo1.PI => uconstr:(e_pi)
+  | R0 => uconstr:(t_zer)
+  | R1 => uconstr:(t_one)
+  | Rplus ?e ?f => let e:=reify e in let f:=reify f in uconstr:(t_add e f)
+  | Rminus ?e ?f => let e:=reify e in let f:=reify f in uconstr:(t_sub e f)
+  | Rmult ?e ?f => let e:=reify e in let f:=reify f in uconstr:(t_mul e f)
+  | Rmult' ?d ?e ?f => let e:=reify e in let f:=reify f in uconstr:(t_mul' d e f)
+  | Rdiv ?e ?f => let e:=reify e in let f:=reify f in uconstr:(t_div e f)
+  | R_sqrt.sqrt ?e => let e:=reify e in uconstr:(t_sqrt e)
+  | Rtrigo_def.cos ?e => let e:=reify e in uconstr:(t_cos e)
+  | Rtrigo_def.sin ?e => let e:=reify e in uconstr:(t_sin e)
+  | Rabs ?e => let e:=reify e in uconstr:(t_abs e)
+  | Q2R ?q => uconstr:(t_fromQ q)
+  | IZR ?z => uconstr:(t_fromZ z)
+  | Rtrigo1.PI => uconstr:(t_pi)
   | RInt ?f ?a ?b =>
-    let a:=ereify a in
-    let b:=ereify b in
+    let a:=reify a in
+    let b:=reify b in
     let fVAR:=reduce (f VAR) in
-    let f:=freify fVAR in
-    uconstr:(e_integrate f a b)
-  | VAR => fail "variable occurs under an unsupported context"
-  | ?e => fail "unrecognised expression:" e
-  end
- with freify f :=
-    lazymatch f with
-  | sem' (fun X => ?e) VAR => e
-  | Rplus ?e ?f => let e:=freify e in let f:=freify f in uconstr:(f_add e f)
-  | Rminus ?e ?f => let e:=freify e in let f:=freify f in uconstr:(f_sub e f)
-  | Rmult ?e ?f => let e:=freify e in let f:=freify f in uconstr:(f_mul e f)
-  | Rmult' ?d ?e ?f => let e:=freify e in let f:=freify f in uconstr:(f_trunc d (f_mul e f))
-  | Rtruncate ?d ?e => let e:=freify e in uconstr:(f_trunc d e)
-  | Rdiv ?e ?f => let e:=freify e in let f:=freify f in uconstr:(f_div e f)
-  | R_sqrt.sqrt ?e => let e:=freify e in uconstr:(f_sqrt e)
-  | set ?p ?e => let e:=freify e in uconstr:(t_set p e)
-  | Rtrigo_def.cos VAR => uconstr:(f_cos)
-  | Rtrigo_def.sin VAR => uconstr:(f_sin)
-  | VAR => uconstr:(f_id)
-  | ?e => let e:=ereify e in uconstr:(f_cst e)
-    end.
-Ltac breify b :=
-  lazymatch b with
-  | sem' (fun X => ?e) => e
+    let f:=reify fVAR in
+    uconstr:(t_integrate f a b)
+  | Rtruncate ?d ?e => let e:=reify e in uconstr:(t_trunc d e)
+  | VAR => uconstr:(t_id)
   | ?e <= ?f <= ?g =>
-    let e:=ereify e in let f:=ereify f in let g:=ereify g in
-    uconstr:(let' f (fun x => b_conj (b_le e x) (b_le x g)))
+    let e:=reify e in let f:=reify f in let g:=reify g in
+    uconstr:(t_let' f (fun x => t_conj (t_le e x) (t_le x g)))
     (* TOREPORT: weird bug if we alpha-rename x into f above (see DAGGER below) *)
   | ?e <= ?f < ?g =>
-    let e:=ereify e in let f:=ereify f in let g:=ereify g in
-    uconstr:(let' f (fun x => b_conj (b_le e x) (b_lt x g)))
+    let e:=reify e in let f:=reify f in let g:=reify g in
+    uconstr:(t_let' f (fun x => t_conj (t_le e x) (t_lt x g)))
   | ?e < ?f <= ?g =>
-    let e:=ereify e in let f:=ereify f in let g:=ereify g in
-    uconstr:(let' f (fun x => b_conj (b_lt e x) (b_le x g)))
+    let e:=reify e in let f:=reify f in let g:=reify g in
+    uconstr:(t_let' f (fun x => t_conj (t_lt e x) (t_le x g)))
   | ?e < ?f <= ?g =>
-    let e:=ereify e in let f:=ereify f in let g:=ereify g in
-    uconstr:(let' f (fun x => b_conj (b_lt e x) (b_lt x g)))
-  | Rle ?e ?f => let e:=ereify e in let f:=ereify f in uconstr:(b_le e f)
-  | Rge ?e ?f => let e:=ereify e in let f:=ereify f in uconstr:(b_ge e f)
-  | Rlt ?e ?f => let e:=ereify e in let f:=ereify f in uconstr:(b_lt e f)
-  | Rgt ?f ?e => let e:=ereify e in let f:=ereify f in uconstr:(b_lt e f)
-  | ?e <> ?f => let e:=ereify e in let f:=ereify f in uconstr:(b_ne e f)
-  | ?b /\ ?c => let b:=breify b in let c:=breify c in uconstr:(b_conj b c)
-  | ?b \/ ?c => let b:=breify b in let c:=breify c in uconstr:(b_disj b c)
-  | set ?p ?e => let e:=breify e in uconstr:(t_set p e)
+    let e:=reify e in let f:=reify f in let g:=reify g in
+    uconstr:(t_let' f (fun x => t_conj (t_lt e x) (t_lt x g)))
+  | Rle ?e ?f => let e:=reify e in let f:=reify f in uconstr:(t_le e f)
+  | Rge ?e ?f => let e:=reify e in let f:=reify f in uconstr:(t_ge e f)
+  | Rlt ?e ?f => let e:=reify e in let f:=reify f in uconstr:(t_lt e f)
+  | Rgt ?f ?e => let e:=reify e in let f:=reify f in uconstr:(t_lt e f)
+  | ?e <> ?f => let e:=reify e in let f:=reify f in uconstr:(t_ne e f)
+  | ?b /\ ?c => let b:=reify b in let c:=reify c in uconstr:(t_conj b c)
+  | ?b \/ ?c => let b:=reify b in let c:=reify c in uconstr:(t_disj b c)
+  | True => uconstr:(t_true)
+  | False => uconstr:(t_false)
   | forall x, ?a <= x <= ?b -> @?p x =>
-    let a:=ereify a in
-    let b:=ereify b in
+    let a:=reify a in
+    let b:=reify b in
     let pVAR:=reduce (p VAR) in
-    let p:=creify pVAR in
-    uconstr:(b_forall_models a b p)
-  | ?e => fail "unrecognised propositional expression:" e
-  end
-    with creify b :=
-  lazymatch b with
-  | sem' (fun X => ?e) VAR => e
-  | ?e < ?f < ?g =>
-    let e:=freify e in let f:=freify f in let g:=freify g in
-    uconstr:(let' f (fun x => c_conj (c_lt e x) (c_lt x g)))
-  | Rlt ?e ?f => let e:=freify e in let f:=freify f in uconstr:(c_lt e f)
-  | ?e <> ?f => let e:=freify e in let f:=freify f in uconstr:(c_ne e f)
-  | ?b /\ ?c => let b:=creify b in let c:=creify c in uconstr:(c_conj b c)
-  | ?b \/ ?c => let b:=creify b in let c:=creify c in uconstr:(c_disj b c)
-  | ?e => let e:=breify e in uconstr:(c_cst e)
-  | set ?p ?e => let e:=creify e in uconstr:(t_set p e)
+    let p:=reify pVAR in
+    uconstr:(t_forall_models a b p)
+  | set ?p ?e => let e:=reify e in uconstr:(t_set p e)
+  (* | ?e => let e:=reify e in uconstr:(t_cst e) *)
+  | ?e => fail "unrecognised expression:" e
   end.
 Ltac reify_real e :=
   let e := reduce e in
-  let e := ereify e in
-  constr:((fun X => e): Term REAL).
+  let e := reify e in
+  constr:((fun X => e): Term ZER REAL).
 Ltac reify_fun e :=
   let e := reduce (e VAR) in
-  let e := freify e in
-  constr:((fun X => e): Term FUN).
+  let e := reify e in
+  constr:((fun X => e): Term ONE REAL).
 Ltac reify_prop e :=
   let e := reduce e in
-  let e := breify e in
-  constr:((fun X => e): Term BOOL).
+  let e := reify e in
+  constr:((fun X => e): Term ZER PROP).
 Ltac reify_pred e :=
-  let e := reduce e in
-  let e := creify e in
-  constr:((fun X => e): Term PRED).
+  let e := reduce (e VAR) in
+  let e := reify e in
+  constr:((fun X => e): Term ONE PROP).
 
 (* tests for the above reification tatics *)
 (*
+Ltac test r c := let e := r c in unify c (sem' e); pose e.
 Goal True.
-  let e := reify_real constr:(Rplus R0 R1) in pose e.
-  let e := reify_real constr:(42) in pose e.
-  let e := reify_real constr:(4.2) in pose e.
-  let e := reify_real constr:(0+1: R) in pose e.
-  let e := reify_real constr:(RInt (fun z => z) R0 R1) in pose e.
-  let e := reify_real constr:(RInt (fun z => R0) R0 R1) in pose e.
-  let e := reify_real constr:(RInt (fun z => R0+z) R0 R1) in pose e.
-  let e := reify_real constr:(RInt (fun z => R0+z) R0 R1) in pose e.
-  let e := reify_real constr:(RInt (@sqrt _) R0 R1) in pose e.
-  let e := reify_real constr:(RInt (@sqrt _ + @sqrt _) R0 R1) in pose e.
-  let e := reify_real constr:(RInt (@sqrt _ *[4] @sqrt _) R0 R1) in pose e.
-  let e := reify_real constr:(RInt (fun x => sqrt x *[4] sqrt x) R0 R1) in pose e.
-  let e := reify_real constr:(RInt (fun x => sqrt x *[4] (set (degree 5) (sqrt x))) R0 R1) in pose e.
-  let e := reify_real constr:(RInt (fun x => sqrt x *[4] (Rtruncate 5 (sqrt x))) R0 R1) in pose e.
-  let e := reify_real constr:(RInt (fun z => R0+z+cos (1/fromZ 2)) R0 R1) in pose e.
-  let f := reify_fun  constr:(fun x: R => x * sqrt x) in pose f.
-  let b := reify_prop constr:(1/2 <= 3 <= 1/2) in pose b. (* DAGGER: double check *)
-  let b := reify_prop constr:(4 <= 5 <= 6) in pose b.
-  let b := reify_prop constr:(4 < 5 /\ 3 <= RInt id 3.3 4.4 <= 18.9) in pose b.
-  let b := reify_prop constr:(4 >= 5) in pose b. 
-  let b := reify_prop constr:(forall x, 4 <= x <= 5 -> x*x < sqrt x) in pose b.
-  let b := reify_prop constr:(set (degree 3) (1/2 <= 3) /\ set (depth 4) (0 <= 1/2)) in pose b.
-  let b := reify_prop constr:(forall x, 2<=x<=cos 2 -> 1/x <> sqrt x) in pose b. 
-  Fail let b := reify_prop constr:(forall x, 2<=x<=cos x -> 1/x <> sqrt x) in pose b. 
+  test reify_real (Rplus R0 R1).
+  test reify_real (42).
+  test reify_real (4.2).
+  test reify_real (0+1: R).
+  test reify_real (RInt (fun z => z) R0 R1).
+  test reify_real (RInt (fun z => R0) R0 R1).
+  test reify_real (RInt (fun z => R0+z) R0 R1).
+  test reify_real (RInt (fun z => R0+z) R0 R1).
+  test reify_real (RInt sqrt R0 R1).
+  test reify_real (RInt (sqrt + sqrt) R0 R1).
+  test reify_real (RInt (sqrt *[4] sqrt) R0 R1).
+  test reify_real (Rtrigo1.PI *[4] Rtrigo1.PI).
+  test reify_real (RInt (fun x => sqrt x *[4] sqrt x) R0 R1).
+  test reify_real (RInt (fun x => sqrt x *[4] (set (degree 5) (sqrt x))) R0 R1).
+  test reify_real (RInt (fun x => sqrt x *[4] (Rtruncate 5 (sqrt x))) R0 R1).
+  test reify_real (RInt (fun z => R0+z+cos (1/fromZ 2)) R0 R1).
+  test reify_fun  (fun x: R => x * sqrt x).
+  test reify_prop (1/2 <= 3 <= 1/2). (* DAGGER: double check *)
+  test reify_prop (4 <= 5 <= 6).
+  test reify_prop (4 < 5 /\ 3 <= RInt id 3.3 4.4 <= 18.9).
+  test reify_prop (4 >= 5). 
+  test reify_prop (forall x, 4 <= x <= 5 -> x*x < sqrt x).
+  test reify_prop (set (degree 3) (1/2 <= 3) /\ set (depth 4) (0 <= 1/2)).
+  test reify_prop (forall x, 2<=x<=cos 2 -> 1/x <> sqrt x). 
+  Fail test reify_prop (forall x, 2<=x<=cos x -> 1/x <> sqrt x). 
   exact I. 
 Qed.
  *)
@@ -298,61 +281,63 @@ Abort.
 
    problem is that this generates useless reformulations of [eq] for the types used in term (sort, Z, Q)
   *)
-Inductive trel X Y (R: forall S, X S -> Y S -> Prop): forall S, @term X S -> @term Y S -> Prop :=
-| re_add: forall x y, trel R x y -> forall x' y', trel R x' y' -> trel R (e_add x x') (e_add y y')
-| re_sub: forall x y, trel R x y -> forall x' y', trel R x' y' -> trel R (e_sub x x') (e_sub y y')
-| re_mul: forall x y, trel R x y -> forall x' y', trel R x' y' -> trel R (e_mul x x') (e_mul y y')
-| re_fromZ: forall z, trel R (e_fromZ z) (e_fromZ z)
-| re_fromQ: forall q, trel R (e_fromQ q) (e_fromQ q)
-| re_zer: trel R e_zer e_zer
-| re_one: trel R e_one e_one
-| re_pi: trel R e_pi e_pi
-| re_div: forall x y, trel R x y -> forall x' y', trel R x' y' -> trel R (e_div x x') (e_div y y')
-| re_sqrt: forall x y, trel R x y -> trel R (e_sqrt x) (e_sqrt y)
-| re_cos: forall x y, trel R x y -> trel R (e_cos x) (e_cos y)
-| re_sin: forall x y, trel R x y -> trel R (e_sin x) (e_sin y)
-| re_abs: forall x y, trel R x y -> trel R (e_abs x) (e_abs y)
-| re_eval: forall x y, trel R x y -> forall x' y', trel R x' y' -> trel R (e_eval x x') (e_eval y y')
-| re_integrate: forall f g, trel R f g -> forall x y, trel R x y -> forall x' y', trel R x' y' -> trel R (e_integrate f x x') (e_integrate g y y')
-| rf_add: forall x y, trel R x y -> forall x' y', trel R x' y' -> trel R (f_add x x') (f_add y y')
-| rf_sub: forall x y, trel R x y -> forall x' y', trel R x' y' -> trel R (f_sub x x') (f_sub y y')
-| rf_mul: forall x y, trel R x y -> forall x' y', trel R x' y' -> trel R (f_mul x x') (f_mul y y')
-| rf_div: forall x y, trel R x y -> forall x' y', trel R x' y' -> trel R (f_div x x') (f_div y y')
-| rf_sqrt: forall x y, trel R x y -> trel R (f_sqrt x) (f_sqrt y)
-| rf_id: trel R f_id f_id
-| rf_cos: trel R f_cos f_cos
-| rf_sin: trel R f_sin f_sin
-| rf_cst: forall x y, trel R x y -> trel R (f_cst x) (f_cst y)
-| rf_trunc: forall d x y, trel R x y -> trel R (f_trunc d x) (f_trunc d y)
-| rb_le: forall x y, trel R x y -> forall x' y', trel R x' y' -> trel R (b_le x x') (b_le y y')
-| rb_ge: forall x y, trel R x y -> forall x' y', trel R x' y' -> trel R (b_ge x x') (b_ge y y')
-| rb_lt: forall x y, trel R x y -> forall x' y', trel R x' y' -> trel R (b_lt x x') (b_lt y y')
-| rb_ne: forall x y, trel R x y -> forall x' y', trel R x' y' -> trel R (b_ne x x') (b_ne y y')
-| rb_disj: forall x y, trel R x y -> forall x' y', trel R x' y' -> trel R (b_disj x x') (b_disj y y')
-| rb_conj: forall x y, trel R x y -> forall x' y', trel R x' y' -> trel R (b_conj x x') (b_conj y y')
-| rb_forall_models: forall x y, trel R x y -> forall x' y', trel R x' y' -> forall h k, trel R h k -> 
-                           trel R (b_forall_models x x' h) (b_forall_models y y' k)
-| rb_forall_bisect: forall x y, trel R x y -> forall x' y', trel R x' y' -> 
-                    forall h k, (forall a b, R REAL a b -> trel R (h a) (k b)) -> 
-                           trel R (b_forall_bisect x x' h) (b_forall_bisect y y' k)
-| rc_lt: forall f g, trel R f g -> forall h k, trel R h k -> trel R (c_lt f h) (c_lt g k)
-| rc_ne: forall f g, trel R f g -> forall h k, trel R h k -> trel R (c_ne f h) (c_ne g k)
-| rc_disj: forall x y, trel R x y -> forall x' y', trel R x' y' -> trel R (c_disj x x') (c_disj y y')
-| rc_conj: forall x y, trel R x y -> forall x' y', trel R x' y' -> trel R (c_conj x x') (c_conj y y')
-| rc_cst: forall x y, trel R x y -> trel R (c_cst x) (c_cst y)
-| rc_forall_bisect: forall x y, trel R x y -> forall x' y', trel R x' y' -> 
-                    forall h k, (forall a b, R REAL a b -> trel R (h a) (k b)) -> 
-                           trel R (c_forall_bisect x x' h) (c_forall_bisect y y' k)
-| rt_set: forall p S x y, trel R x y -> trel R (@t_set _ S p x) (@t_set _ S p y)
-| rt_var: forall S x y, R S x y -> trel R (t_var x) (t_var y)
-| rt_let: forall S T x y h k, trel R x y -> (forall a b, R S a b -> trel R (h a) (k b)) -> trel R (t_let x h) (@t_let _ _ T y k).
+Inductive trel X Y (R: forall D C, X D C -> Y D C -> Prop): forall D C, @term X D C -> @term Y D C -> Prop :=
+| t_addR: forall D x y, trel R x y -> forall x' y', trel R x' y' -> trel R (D:=D) (t_add x x') (t_add y y')
+| t_subR: forall D x y, trel R x y -> forall x' y', trel R x' y' -> trel R (D:=D) (t_sub x x') (t_sub y y')
+| t_mulR: forall D x y, trel R x y -> forall x' y', trel R x' y' -> trel R (D:=D) (t_mul x x') (t_mul y y')
+| t_mul'R: forall D d x y, trel R x y -> forall x' y', trel R x' y' -> trel R (D:=D) (t_mul' d x x') (t_mul' d y y')
+| t_divR: forall D x y, trel R x y -> forall x' y', trel R x' y' -> trel R (D:=D) (t_div x x') (t_div y y')
+| t_sqrtR: forall D x y, trel R x y -> trel R (D:=D) (t_sqrt x) (t_sqrt y)
+| t_cosR: forall D x y, trel R x y -> trel R (D:=D) (t_cos x) (t_cos y)
+| t_sinR: forall D x y, trel R x y -> trel R (D:=D) (t_sin x) (t_sin y)
+| t_absR: forall D x y, trel R x y -> trel R (D:=D) (t_abs x) (t_abs y)
+| t_fromZR: forall D z, trel R (D:=D) (t_fromZ z) (t_fromZ z)
+| t_fromQR: forall D q, trel R (D:=D) (t_fromQ q) (t_fromQ q)
+| t_zerR: forall D, trel R (D:=D) t_zer t_zer
+| t_oneR: forall D, trel R (D:=D) t_one t_one
+| t_piR: forall D, trel R (D:=D) t_pi t_pi
+| t_idR: trel R t_id t_id
+| t_appR: forall x y, trel R x y -> forall x' y', trel R x' y' -> trel R (t_app x x') (t_app y y')
+| t_integrateR: forall f g, trel R f g -> forall x y, trel R x y -> forall x' y', trel R x' y' -> trel R (t_integrate f x x') (t_integrate g y y')
+| t_cstR: forall C x y, trel R x y -> trel R (C:=C) (t_cst x) (t_cst y)
+| t_truncR: forall d x y, trel R x y -> trel R (t_trunc d x) (t_trunc d y)
+| t_leR: forall D x y, trel R x y -> forall x' y', trel R x' y' -> trel R (D:=D) (t_le x x') (t_le y y')
+| t_geR: forall D x y, trel R x y -> forall x' y', trel R x' y' -> trel R (D:=D) (t_ge x x') (t_ge y y')
+| t_ltR: forall D x y, trel R x y -> forall x' y', trel R x' y' -> trel R (D:=D) (t_lt x x') (t_lt y y')
+| t_neR: forall D x y, trel R x y -> forall x' y', trel R x' y' -> trel R (D:=D) (t_ne x x') (t_ne y y')
+| t_disjR: forall D x y, trel R x y -> forall x' y', trel R x' y' -> trel R (D:=D) (t_disj x x') (t_disj y y')
+| t_conjR: forall D x y, trel R x y -> forall x' y', trel R x' y' -> trel R (D:=D) (t_conj x x') (t_conj y y')
+| t_trueR: forall D, trel R (D:=D) t_true t_true
+| t_falseR: forall D, trel R (D:=D) t_false t_false
+| t_forall_modelsR: forall x y, trel R x y -> forall x' y', trel R x' y' -> forall h k, trel R h k -> 
+                           trel R (t_forall_models x x' h) (t_forall_models y y' k)
+| t_forall_bisectR: forall D x y, trel R x y -> forall x' y', trel R x' y' -> 
+                    forall h k, (forall a b, R ZER REAL a b -> trel R (h a) (k b)) -> 
+                           trel R (D:=D) (t_forall_bisect x x' h) (t_forall_bisect y y' k)
+| t_setR: forall p D C x y, trel R x y -> trel R (@t_set _ D C p x) (@t_set _ D C p y)
+| t_varR: forall D C x y, R D C x y -> trel R (t_var x) (t_var y)
+| t_letR: forall D C F E x y h k, trel R x y -> (forall a b, R D C a b -> trel R (h a) (k b)) -> trel R (t_let x h) (@t_let _ _ _ F E y k).
 
 (** all (closed) terms are parametric in the following sense, 
-    but this cannot be proved once and for all. Given a concrete closed term, it is however trivial to prove its parametricity (tactic: repeat (constructor; auto)) 
+    but this cannot be proved once and for all. Given a concrete closed term, it is however trivial to prove its parametricity.
     once a closed term has been proved parametric, one can prove facts by induction on this term
     (see lemmas [Static.correct] and [Dynamic.correct] below) *)
-Definition parametric S (u: Term S) :=
-  forall X Y (R: forall S, X S -> Y S -> Prop), trel R (u X) (u Y).
+Definition parametric D C (u: Term D C) :=
+  forall X Y (R: forall D C, X D C -> Y D C -> Prop), trel R (u X) (u Y).
+Ltac prove_parametric := repeat (constructor; auto).  
+  
+
+
+Definition is_id X D C (t: @term X D C) :=
+  match t with t_id => true | _ => false end.
+Definition often_id X D C: @term X D C -> @term X D C :=
+  match D,C with ONE,REAL => fun _ => t_id | _,_ => id end.
+Lemma is_idE' X D C (t: @term X D C): impl (is_id t) (t=often_id t).
+Proof. case: t=>//=. by constructor. Qed.
+Lemma is_idE X (t: @term X ONE REAL): impl (is_id t) (t=t_id).
+Proof. apply is_idE'. Qed.
+Lemma is_idR X Y R D C s t: @trel X Y R D C s t -> is_id s = is_id t.
+Proof. by case. Qed.
 
 
 (** ** static evaluation function *)
@@ -360,102 +345,117 @@ Definition parametric S (u: Term S) :=
 Module Static.
 Section s.
 
-Context {N: NBH} (MO: ModelOps) (D: Domain) (M: Model MO dlo dhi). 
+Context {N: NBH} (MO: ModelOps) (Do: Domain) (M: Model MO dlo dhi). 
 
 
 (** interpretation of expressions using intervals / models / booleans *)
-Definition sval S :=
-  match S with
-  | REAL => E II
-  | FUN => E MM
-  | BOOL => E bool
-  | PRED => E bool
+Definition sval D C :=
+  match C, D with
+  | REAL,ZER => E II
+  | REAL,ONE => E MM
+  | PROP,_ => E bool
   end.
-Fixpoint Sem (p: prms) S (t: @term sval S): sval S :=
-  match t in term S return sval S with
-  | e_add e f => e_map2 (@add _) (Sem p e) (Sem p f)
-  | e_sub e f => e_map2 (@sub _) (Sem p e) (Sem p f)
-  | e_mul e f => e_map2 (@mul _) (Sem p e) (Sem p f)
-  | e_div e f => e_map2 (@div _) (Sem p e) (Sem p f)
-  | e_sqrt e => e_map (@sqrt _) (Sem p e)
-  | e_cos e => e_map (@cos _) (Sem p e)
-  | e_sin e => e_map (@sin _) (Sem p e)
-  | e_abs e => e_map (@abs _) (Sem p e)
-  | e_fromQ q => ret (fromQ q)
-  | e_fromZ z => ret (fromZ z)
-  | e_pi => ret pi
-  | e_zer => ret 0
-  | e_one => ret 1
-  | e_eval f x => 
+Fixpoint Sem (p: prms) D C (t: @term sval D C): sval D C :=
+  match t in term D C return sval D C with
+  | t_add (ZER|ONE) e f => e_map2 add (Sem p e) (Sem p f)
+  | t_sub (ZER|ONE) e f => e_map2 sub (Sem p e) (Sem p f)
+  | t_mul (ZER|ONE) e f => e_map2 mul (Sem p e) (Sem p f)
+  | t_mul' (ZER|ONE) d e f => e_map2 (mul' d) (Sem p e) (Sem p f)
+  | t_zer (ZER|ONE) => ret 0
+  | t_one (ZER|ONE) => ret 1
+  | t_div ZER e f => e_map2 div (Sem p e) (Sem p f)
+  | t_sqrt ZER e => e_map sqrt (Sem p e)
+  | t_cos ZER e => e_map cos (Sem p e)
+  | t_sin ZER e => e_map sin (Sem p e)
+  | t_abs ZER e => e_map abs (Sem p e)
+  | t_fromQ ZER z => ret (fromQ z)
+  | t_fromZ ZER z => ret (fromZ z)
+  | t_pi ZER => ret pi
+  | t_div ONE e f => LET e ::= Sem p e IN LET f ::= Sem p f IN mdiv (p_deg p) (p_trunc p) e f
+  | t_sqrt ONE e => LET e ::= Sem p e IN msqrt (p_deg p) (p_trunc p) e
+  | t_cos ONE e => if is_id e then mcos else err "cosine cannot be composed in models"
+  | t_sin ONE e => if is_id e then msin else err "sine cannot be composed in models"
+  | t_abs ONE e => err "absolute value not supported in models"
+  | t_fromQ ONE q => ret (mcst (fromQ q))
+  | t_fromZ ONE z => ret (mcst (fromZ z))
+  | t_pi ONE => ret (mcst pi)
+  | t_id => mid
+  | t_app f x => 
       LET f ::= Sem p f IN
       LET x ::= Sem p x IN 
       meval f x
-  | e_integrate f a b => 
+  | t_integrate f a b => 
       LET f ::= Sem p f IN 
       LET a ::= Sem p a IN 
       LET b ::= Sem p b IN 
       mintegrate f (Some a) (Some b)
-  | f_add e f => e_map2 (@add _) (Sem p e) (Sem p f)
-  | f_sub e f => e_map2 (@sub _) (Sem p e) (Sem p f)
-  | f_mul e f => e_map2 (@mul _) (Sem p e) (Sem p f)
-  | f_div e f => LET e ::= Sem p e IN LET f ::= Sem p f IN mdiv (p_deg p) (p_trunc p) e f
-  | f_sqrt e => LET e ::= Sem p e IN msqrt (p_deg p) (p_trunc p) e
-  | f_id => mid
-  | f_cos => mcos
-  | f_sin => msin
-  | f_cst e => e_map mcst (Sem p e)
-  | f_trunc d e => e_map (mtruncate d) (Sem p e)
-  | b_le e f => e_map2 is_le (Sem p e) (Sem p f)
-  | b_ge e f => e_map2 is_ge (Sem p e) (Sem p f)
-  | b_lt e f => e_map2 is_lt (Sem p e) (Sem p f)
-  | b_ne e f => e_map2 is_ne (Sem p e) (Sem p f)
-  | b_disj b c | c_disj b c => Eor (Sem p b) (fun _ => Sem p c)
-  | b_conj b c | c_conj b c => Eand (Sem p b) (fun _ => Sem p c)
-  | c_lt f g => LET f ::= Sem p f IN LET g ::= Sem p g IN mlt (p_deg p) f g
-  | c_ne f g => e_map2 (mne (p_deg p)) (Sem p f) (Sem p g)
-  | c_cst b => Sem p b
-  | c_forall_bisect a b k 
-  | b_forall_bisect a b k => 
+  | t_cst REAL e => e_map mcst (Sem p e)
+  | t_cst PROP e => Sem p e
+  | t_trunc d e => e_map (mtruncate d) (Sem p e)
+  | t_le ZER e f => e_map2 is_le (Sem p e) (Sem p f)
+  | t_ge ZER e f => e_map2 is_ge (Sem p e) (Sem p f)
+  | t_lt ZER e f => e_map2 is_lt (Sem p e) (Sem p f)
+  | t_ne ZER e f => e_map2 is_ne (Sem p e) (Sem p f)
+  | t_disj _ b c => Eor (Sem p b) (fun _ => Sem p c)
+  | t_conj _ b c => Eand (Sem p b) (fun _ => Sem p c)
+  | t_true _ => ret true
+  | t_false _ => ret false
+  | t_le ONE f g =>
+      LET f ::= Sem p f IN LET g ::= Sem p g IN mle (p_deg p) f g
+  | t_ge ONE f g =>
+      LET f ::= Sem p f IN LET g ::= Sem p g IN mge (p_deg p) f g
+  | t_lt ONE f g =>
+      LET f ::= Sem p f IN LET g ::= Sem p g IN mlt (p_deg p) f g
+  | t_ne ONE f g => e_map2 (mne (p_deg p)) (Sem p f) (Sem p g)
+  | t_forall_bisect ZER a b k => 
       LET a ::= Sem p a IN
       LET b ::= Sem p b IN
       bisect (p_depth p) (fun x => Sem p (k (ret x))) (interval a b)
-  | b_forall_models a b k => 
+  | t_forall_bisect ONE a b k => 
+      LET a ::= Sem p a IN
+      LET b ::= Sem p b IN
+      bisect (p_depth p) (fun x => Sem p (k (ret x))) (interval (mrange a) (mrange b))
+  | t_forall_models a b k => 
       LET a ::= Sem p a IN
       LET b ::= Sem p b IN
       if ~~is_le dlo a then err "model comparison: lower bound beyond domain" else
       if ~~is_le b dhi then err "model comparison: upper bound beyond domain" else
       Sem p k
-  | t_set _ q x => Sem (set_prm q p) x
-  | t_var _ x => x
-  | t_let _ _ x k => Sem p (k (Sem p x))
+  | t_set _ _ q x => Sem (set_prm q p) x
+  | t_var _ _ x => x
+  | t_let _ _ _ _ x k => Sem p (k (Sem p x))
   end.
-Definition Sem' p S (u: Term S): sval S := Sem p (u sval).
+Definition Sem' p D C (u: Term D C): sval D C := Sem p (u sval).
 
 (** correctness of the above semantics
     the key lemma, [correct], is proved by induction on the parametricity relation *)
-Definition cval S: sval S -> rval S -> Prop :=
-  match S with
-  | REAL => EP' contains
-  | FUN  => EP' mcontains
-  | BOOL => Eimpl
-  | PRED => fun b p => Eimpl b (forall x, dlo <= x <= dhi -> p x)
+Definition cval D C: sval D C -> rval D C -> Prop :=
+  match D,C with
+  | ZER,REAL => EP' contains
+  | ONE,REAL  => EP' mcontains
+  | ZER,PROP => Eimpl
+  | ONE,PROP => fun b p => Eimpl b (forall x, dlo <= x <= dhi -> p x)
   end.
-Lemma correct S (u: term S) (v: term S): trel cval u v -> forall d, cval (Sem d u) (sem v).
+Lemma correct D C (u: term D C) (v: term D C): trel cval u v -> forall d, cval (Sem d u) (sem v).
 Proof.
-  induction 1; intro deg; cbn in *=>//.
-  - eapply ep_map2; eauto. rel. 
-  - eapply ep_map2; eauto. rel. 
-  - eapply ep_map2; eauto. rel. 
-  - constructor. rel. 
-  - constructor. apply fromQR. 
-  - constructor. rel. 
-  - constructor. rel. 
-  - constructor. rel.
-  - eapply ep_map2; eauto. rel. 
-  - eapply ep_map; eauto. rel. 
-  - eapply ep_map; eauto. rel. 
-  - eapply ep_map; eauto. rel. 
-  - eapply ep_map; eauto. rel. 
+  induction 1=>ps/=; 
+                 lazymatch goal with
+                 | |- context [match ?x with _ => _ end] => destruct x
+                 | _ => idtac
+                 end;
+    cbn in *=>//; try ((eapply ep_map || eapply ep_map2 || constructor); eauto; rel).
+  - eapply ep_map2; eauto. unfold Rmult'; rel. 
+  - eapply ep_bind=>[F Ff|]; eauto. 
+    eapply ep_bind=>[G Gg|]; eauto.
+    by apply mdivR.
+  - eapply ep_bind=>[F Ff|]; eauto.
+    by apply msqrtR.
+  - move: (is_idR H). case is_idE=>//. case is_idE=>//-> _ _. apply mcosR. 
+  - move: (is_idR H). case is_idE=>//. case is_idE=>//-> _ _. apply msinR. 
+  - constructor. apply: mcstR; rel.
+  - constructor. rewrite /f_unr/f_cst/=. apply: mcstR; rel.
+  - constructor. apply: mcstR; rel.
+  - apply midR.
   - eapply ep_bind=>[F Ff|]; eauto. 
     eapply ep_bind=>[X Xx|]; eauto.
     by apply mevalR.
@@ -463,74 +463,73 @@ Proof.
     eapply ep_bind=>[A Aa|]; eauto.  
     eapply ep_bind=>[B Bb|]; eauto.  
     apply mintegrateR; rel. 
-  - eapply ep_map2; eauto. intros. by apply: addR.
-  - eapply ep_map2; eauto. intros. by apply: subR.
-  - eapply ep_map2; eauto. intros. by apply: mulR.
+  - case IHtrel=>//b Hb. constructor. case Hb=>//. by constructor. 
+  - eapply ep_map; eauto=>*. by apply mtruncateR.
+  - eapply ep_map2; eauto=>??. case is_leE=>//. auto.  
   - eapply ep_bind=>[F Ff|]; eauto. 
-    eapply ep_bind=>[G Gg|]; eauto.
-    by apply mdivR.
-  - eapply ep_bind=>[F Ff|]; eauto.
-    by apply msqrtR.
-  - apply midR.
-  - apply mcosR.
-  - apply msinR.
-  - eapply ep_map; eauto. intros. by apply mcstR.
-  - eapply ep_map; eauto. intros. by apply mtruncateR.
-  - eapply ep_map2; eauto. intros ??. case is_leE=>//. auto.  
-  - eapply ep_map2; eauto. intros ??. case is_geE=>//. auto. 
-  - eapply ep_map2; eauto. intros ??. case is_ltE=>//. auto.
-  - eapply ep_map2; eauto. intros ??. case is_neE=>//. auto.
-  - by apply Eimpl_or.
-  - by apply Eimpl_and.
+    eapply ep_bind=>[X Xx|]; eauto.
+    by apply mleE.
+  - eapply ep_map2; eauto=>??. case is_geE=>//. auto.  
+  - eapply ep_bind=>[F Ff|]; eauto. 
+    eapply ep_bind=>[X Xx|]; eauto.
+    by apply mgeE.
+  - eapply ep_map2; eauto=>??. case is_ltE=>//. auto.  
+  - eapply ep_bind=>[F Ff|]; eauto. 
+    eapply ep_bind=>[X Xx|]; eauto.
+    by apply mltE.
+  - eapply ep_map2; eauto=>??. case is_neE=>//. auto.  
+  - eapply ep_bind=>[F Ff|]; eauto. 
+    eapply ep_bind=>[X Xx|]; eauto.
+    constructor. by apply mneE.
+  - apply Eimpl_or'.
+    eapply Eimpl_impl. 2: apply IHtrel1. clear; auto. 
+    eapply Eimpl_impl. 2: apply IHtrel2. clear; auto.     
+  - apply Eimpl_or'.
+    eapply Eimpl_impl. 2: apply IHtrel1. clear; auto. 
+    eapply Eimpl_impl. 2: apply IHtrel2. clear; auto. 
+  - eauto using Eimpl_and'.
+  - eauto using Eimpl_and'.
   - eapply ep_bind=>[A HA|]; eauto.
     eapply ep_bind=>[B HB|]; eauto.
     case is_leE=>//=Ha. 
     case is_leE=>//=Hb.
-    move: (IHtrel3 deg). apply Eimpl_impl=>E r ?. apply E. 
+    move: (IHtrel3 ps). apply Eimpl_impl=>E r ?. apply E. 
     specialize (Ha _ _ dloR HA).
     specialize (Hb _ _ HB dhiR).
     cbn in *. lra. 
   - eapply ep_bind=>[A HA|]; eauto.
     eapply ep_bind=>[B HB|]; eauto.
     eapply Eimpl_impl. 2: apply bisectE.
-    move=>K z Hz. apply (K z). by eapply intervalE; eauto.
-    move=>X. apply Eimpl_forall=>z. apply Eimpl_forall=>Hz. by auto.
-  - eapply ep_bind=>[F Ff|]; eauto. 
-    eapply ep_bind=>[G Gg|]; eauto.
-    by apply mltE.
-  - eapply ep_map2; eauto=>????. by apply mneE. 
-  - apply Eimpl_or'.
-    eapply Eimpl_impl. 2: apply IHtrel1. clear; auto. 
-    eapply Eimpl_impl. 2: apply IHtrel2. clear; auto. 
-  - eauto using Eimpl_and'.
-  - eauto using Eimpl_impl. 
+    2: { move=>X. apply Eimpl_forall=>z. apply Eimpl_forall=>Hz. apply H2; eauto. } 
+    move=>K z Hz. apply K=>//. by eapply intervalE; eauto.
   - eapply ep_bind=>[A HA|]; eauto.
     eapply ep_bind=>[B HB|]; eauto.
     eapply Eimpl_impl. 2: apply bisectE.
     2: { move=>X. apply Eimpl_forall=>z. apply Eimpl_forall=>Hz. apply H2; eauto. } 
-    move=>K z Hz t Ht. apply K=>//. by eapply intervalE; eauto.
+    move=>K z Hz t Ht. apply K=>//.
+    by eapply intervalE; eauto; apply mrangeR.
   - auto. 
 Qed.
 
 (** correctness on parametric (closed) terms follows *)
-Lemma Correct: forall p S (u: Term S), parametric u -> cval (Sem' p u) (sem' u).
-Proof. intros p S u U. apply correct, U. Qed.
+Lemma Correct: forall p D C (u: Term D C), parametric u -> cval (Sem' p u) (sem' u).
+Proof. move=>*. by apply correct. Qed.
 
   
 (** small corollary, useful to obtain a tactic in tactic.v *)
-Lemma check p (b: Term BOOL):
+Lemma check p (b: Term ZER PROP):
   parametric b ->
   (let b := Sem' p b in
    match b with ret b => is_true b | err s => False end) ->
   sem' b.
 Proof.
-  move: (@Correct p BOOL)=>/= C B.
+  move: (@Correct p ZER PROP)=>/= C B.
   case C=>//a. apply implE. 
 Qed.
 
 End s.
 Arguments check {_ _ _ _} _ _ _ _.
-Arguments Sem {_} _ _ [_] _.
+Arguments Sem {_} _ _ [_ _] _.
 
 End Static.
 
@@ -543,194 +542,204 @@ Section s.
 Context {N: NBH} (MO: II -> II -> ModelOps) (M: forall D: Domain, Model (MO dlo dhi) dlo dhi).
 
 (** interpretation of expressions using intervals / models / booleans *)
-Definition sval S :=
-  match S with
-  | REAL => E II
-  | FUN => (forall MO: ModelOps, E MM)
-  | BOOL => E bool
-  | PRED => (forall MO: ModelOps, E bool)
+Definition sval D C :=
+  match D,C with
+  | ZER,REAL => E II
+  | ONE,REAL => (forall MO: ModelOps, E MM)
+  | ZER,PROP => E bool
+  | ONE,PROP => (forall MO: ModelOps, E bool)
   end.
-Fixpoint Sem (p: prms) S (t: @term sval S): sval S :=
-  match t in term S return sval S with
-  | e_add e f => e_map2 (@add _) (Sem p e) (Sem p f)
-  | e_sub e f => e_map2 (@sub _) (Sem p e) (Sem p f)
-  | e_mul e f => e_map2 (@mul _) (Sem p e) (Sem p f)
-  | e_div e f => e_map2 (@div _) (Sem p e) (Sem p f)
-  | e_sqrt e => e_map (@sqrt _) (Sem p e)
-  | e_cos e => e_map (@cos _) (Sem p e)
-  | e_sin e => e_map (@sin _) (Sem p e)
-  | e_abs e => e_map (@abs _) (Sem p e)
-  | e_fromQ q => ret (fromQ q)
-  | e_fromZ z => ret (fromZ z)
-  | e_pi => ret pi
-  | e_zer => ret 0
-  | e_one => ret 1
-  | e_eval f x => err "evaluation not yet supported in dynamic mode"
-      (* LET f ::= Sem p f IN *)
-      (* LET x ::= Sem p x IN  *)
-      (* meval f x *)
-  | e_integrate f a b => 
+Fixpoint Sem (p: prms) D C (t: @term sval D C): sval D C :=
+  match t in term D C return sval D C with
+  | t_add ZER e f => e_map2 add (Sem p e) (Sem p f)
+  | t_sub ZER e f => e_map2 sub (Sem p e) (Sem p f)
+  | t_mul ZER e f => e_map2 mul (Sem p e) (Sem p f)
+  | t_mul' ZER d e f => e_map2 (mul' d) (Sem p e) (Sem p f)
+  | t_zer ZER => ret 0
+  | t_one ZER => ret 1
+  | t_div ZER e f => e_map2 div (Sem p e) (Sem p f)
+  | t_sqrt ZER e => e_map sqrt (Sem p e)
+  | t_cos ZER e => e_map cos (Sem p e)
+  | t_sin ZER e => e_map sin (Sem p e)
+  | t_abs ZER e => e_map abs (Sem p e)
+  | t_fromQ ZER z => ret (fromQ z)
+  | t_fromZ ZER z => ret (fromZ z)
+  | t_pi ZER => ret pi
+  | t_add ONE e f => fun MO => e_map2 add (Sem p e MO) (Sem p f MO)
+  | t_sub ONE e f => fun MO => e_map2 sub (Sem p e MO) (Sem p f MO)
+  | t_mul ONE e f => fun MO => e_map2 mul (Sem p e MO) (Sem p f MO)
+  | t_mul' ONE d e f => fun MO => e_map2 (mul' d) (Sem p e MO) (Sem p f MO)
+  | t_zer ONE => fun MO => ret 0
+  | t_one ONE => fun MO => ret 1
+  | t_div ONE e f => fun MO => LET e ::= Sem p e MO IN LET f ::= Sem p f MO IN mdiv (p_deg p) (p_trunc p) e f
+  | t_sqrt ONE e => fun MO => LET e ::= Sem p e MO IN msqrt (p_deg p) (p_trunc p) e
+  | t_cos ONE e => fun MO => if is_id e then mcos else err "cosine cannot be composed in models"
+  | t_sin ONE e => fun MO => if is_id e then msin else err "sine cannot be composed in models"
+  | t_abs ONE e => fun MO => err "absolute value not supported in models"
+  | t_fromQ ONE q => fun MO => ret (mcst (fromQ q))
+  | t_fromZ ONE z => fun MO => ret (mcst (fromZ z))
+  | t_pi ONE => fun MO => ret (mcst pi)
+  | t_id => fun MO => mid
+  | t_app f x => err "application not yet supported in dynamic mode"
+  | t_integrate f a b => 
       LET a ::= Sem p a IN 
       LET b ::= Sem p b IN 
       if ~~ is_lt a b then err "dynamic: integral does not yield a valid domain" else
       LET f ::= Sem p f (MO a b) IN 
       mintegrate f None None
-  | f_add e f => fun MO => e_map2 (@add _) (Sem p e MO) (Sem p f MO)
-  | f_sub e f => fun MO => e_map2 (@sub _) (Sem p e MO) (Sem p f MO)
-  | f_mul e f => fun MO => e_map2 (@mul _) (Sem p e MO) (Sem p f MO)
-  | f_div e f => fun MO => LET e ::= Sem p e MO IN LET f ::= Sem p f MO IN mdiv (p_deg p) (p_trunc p) e f
-  | f_sqrt e => fun MO => LET e ::= Sem p e MO IN msqrt (p_deg p) (p_trunc p) e
-  | f_id => fun MO => mid
-  | f_cos => fun MO => mcos
-  | f_sin => fun MO => msin
-  | f_cst e => fun MO => e_map mcst (Sem p e)
-  | f_trunc d e => fun MO => e_map (mtruncate d) (Sem p e MO)
-  | b_le e f => e_map2 is_le (Sem p e) (Sem p f)
-  | b_ge e f => e_map2 is_ge (Sem p e) (Sem p f) 
-  | b_lt e f => e_map2 is_lt (Sem p e) (Sem p f)
-  | b_ne e f => e_map2 is_ne (Sem p e) (Sem p f)
-  | b_disj b c => Eor (Sem p b) (fun _ => Sem p c)
-  | b_conj b c => Eand (Sem p b) (fun _ => Sem p c)
-  | b_forall_models a b k => 
+  | t_cst REAL e => fun MO => e_map mcst (Sem p e)
+  | t_cst PROP e => fun MO => Sem p e
+  | t_trunc d e => fun MO => e_map (mtruncate d) (Sem p e MO)
+  | t_le ZER e f => e_map2 is_le (Sem p e) (Sem p f)
+  | t_ge ZER e f => e_map2 is_ge (Sem p e) (Sem p f)
+  | t_lt ZER e f => e_map2 is_lt (Sem p e) (Sem p f)
+  | t_ne ZER e f => e_map2 is_ne (Sem p e) (Sem p f)
+  | t_disj ZER b c => Eor (Sem p b) (fun _ => Sem p c)
+  | t_conj ZER b c => Eand (Sem p b) (fun _ => Sem p c)
+  | t_true ZER => ret true
+  | t_false ZER => ret false
+  | t_disj ONE b c => fun MO => Eor (Sem p b MO) (fun _ => Sem p c MO)
+  | t_conj ONE b c => fun MO => Eand (Sem p b MO) (fun _ => Sem p c MO)
+  | t_true ONE => fun MO => ret true
+  | t_false ONE => fun MO => ret false
+  | t_lt ONE f g =>
+      fun MO => LET f ::= Sem p f MO IN LET g ::= Sem p g MO IN mlt (p_deg p) f g
+  | t_le ONE f g =>
+      fun MO => LET f ::= Sem p f MO IN LET g ::= Sem p g MO IN mle (p_deg p) f g
+  | t_ge ONE f g =>
+      fun MO => LET f ::= Sem p f MO IN LET g ::= Sem p g MO IN mge (p_deg p) f g
+  | t_ne ONE f g => 
+      fun MO => e_map2 (mne (p_deg p)) (Sem p f MO) (Sem p g MO)
+  | t_forall_bisect ZER a b k => 
+      LET a ::= Sem p a IN
+      LET b ::= Sem p b IN
+      bisect (p_depth p) (fun x => Sem p (k (ret x))) (interval a b)
+  | t_forall_bisect ONE a b k => 
+      fun MO =>
+      LET a ::= Sem p a MO IN
+      LET b ::= Sem p b MO IN
+      bisect (p_depth p) (fun x => Sem p (k (ret x)) MO) (interval (mrange a) (mrange b))
+  | t_forall_models a b k => 
       LET a ::= Sem p a IN
       LET b ::= Sem p b IN
       bisect2 (p_depth p) (fun a b =>
                              if ~~ is_lt a b then err "invalid domain" else
                                Sem p k (MO a b)) a b
-  | b_forall_bisect a b k =>
-      LET a ::= Sem p a IN
-      LET b ::= Sem p b IN
-      bisect (p_depth p) (fun ab => Sem p (k (ret ab))) (interval a b)
-  | c_lt f g =>
-      fun M => 
-      LET f ::= Sem p f M IN 
-      LET g ::= Sem p g M IN
-      mlt (p_deg p) f g
-  | c_ne f g =>
-      fun M => 
-      LET f ::= Sem p f M IN 
-      LET g ::= Sem p g M IN
-      ret (mne (p_deg p) f g)
-  | c_disj b c => fun M => Eor (Sem p b M) (fun _ => Sem p c M)
-  | c_conj b c => fun M => Eand (Sem p b M) (fun _ => Sem p c M)
-  | c_cst b => fun _ => Sem p b
-  | c_forall_bisect a b k =>
-      fun M =>
-      LET a ::= Sem p a IN
-      LET b ::= Sem p b IN
-      bisect (p_depth p) (fun ab => Sem p (k (ret ab)) M) (interval a b)
-  | t_set _ q x => Sem (set_prm q p) x
-  | t_var _ x => x
-  | t_let _ _ x k => Sem p (k (Sem p x))
+  | t_set _ _ q x => Sem (set_prm q p) x
+  | t_var _ _ x => x
+  | t_let _ _ _ _ x k => Sem p (k (Sem p x))
   end.
-Definition Sem' p S (u: Term S): sval S := Sem p (u sval).
+Definition Sem' p D C (u: Term D C): sval D C := Sem p (u sval).
 
 (** correctness of the above semantics
     the key lemma, [correct], is proved by induction on the parametricity relation *)
-Definition cval S: sval S -> rval S -> Prop :=
-  match S with
-  | REAL => EP' contains
-  | FUN  => fun F f => forall MO a b (M: Model MO a b), EP' M (F MO) f
-  | BOOL => Eimpl
-  | PRED => fun P p => forall MO a b (M: Model MO a b), Eimpl (P MO) (forall x, a <= x <= b -> p x)
+Definition cval D C: sval D C -> rval D C -> Prop :=
+  match D,C with
+  | ZER,REAL => EP' contains
+  | ONE,REAL => fun F f => forall MO a b (M: Model MO a b), EP' M (F MO) f
+  | ZER,PROP => Eimpl
+  | ONE,PROP => fun P p => forall MO a b (M: Model MO a b), Eimpl (P MO) (forall x, a <= x <= b -> p x)
   end.
-Lemma correct S (u: term S) (v: term S): trel cval u v -> forall p, cval (Sem p u) (sem v).
+Lemma correct D C (u: term D C) (v: term D C): trel cval u v -> forall p, cval (Sem p u) (sem v).
+
 Proof.
-  induction 1; intro ps; cbn -[RInt] in *;
-    try (intros MO' a b M';
-         try specialize (IHtrel  _ _ _ M');
-         try (specialize (IHtrel1  _ _ _ M'); specialize (IHtrel2  _ _ _ M'))); trivial.
-  - eapply ep_map2; eauto. rel. 
-  - eapply ep_map2; eauto. rel. 
-  - eapply ep_map2; eauto. rel. 
-  - constructor. rel. 
-  - constructor. apply fromQR. 
-  - constructor. rel. 
-  - constructor. rel. 
-  - constructor. rel.
-  - eapply ep_map2; eauto. rel. 
-  - eapply ep_map; eauto. rel. 
-  - eapply ep_map; eauto. rel. 
-  - eapply ep_map; eauto. rel. 
-  - eapply ep_map; eauto. rel. 
+  induction 1=>ps/=; 
+                 lazymatch goal with
+                 | |- context [match ?x with _ => _ end] => destruct x
+                 | _ => idtac
+                 end;
+    cbn -[RInt] in *=>//; try intros MO' a b M'; 
+    try ((eapply ep_map || eapply ep_map2 || constructor); eauto; rel).
+  - eapply ep_map2; eauto. unfold Rmult'; rel. 
+  - eapply ep_bind=>[F Ff|]; eauto. 
+    eapply ep_bind=>[G Gg|]; eauto.
+    by apply mdivR.
+  - eapply ep_bind=>[F Ff|]; eauto.
+    by apply msqrtR.
+  - move: (is_idR H). case is_idE=>//. case is_idE=>//-> _ _. apply mcosR. 
+  - move: (is_idR H). case is_idE=>//. case is_idE=>//-> _ _. apply msinR. 
+  - constructor. apply: mcstR; rel.
+  - constructor. rewrite /f_unr/f_cst/=. apply: mcstR; rel.
+  - constructor. apply: mcstR; rel.
+  - apply midR.
   - eapply ep_bind=>[A Aa|]; eauto.  
     eapply ep_bind=>[B Bb|]; eauto.  
     case_eq (is_lt A B)=>//=ab. 
     specialize (IHtrel1 ps _ _ _ (M (DfromI2 Aa Bb ab))).
     eapply ep_bind=>[F Ff|]; eauto.
     eapply mintegrateR; first apply Ff; by constructor. 
-  - eapply ep_map2; eauto. intros. by apply: addR.
-  - eapply ep_map2; eauto. intros. by apply: subR.
-  - eapply ep_map2; eauto. intros. by apply: mulR.
+  - case IHtrel=>//c Hc. constructor. case Hc=>//. by constructor. 
+  - eapply ep_map; eauto=>*. by apply mtruncateR.
+  - eapply ep_map2; eauto=>??. case is_leE=>//. auto.  
   - eapply ep_bind=>[F Ff|]; eauto. 
-    eapply ep_bind=>[G Gg|]; eauto.
-    by apply mdivR.
-  - eapply ep_bind=>[F Ff|]; eauto.
-    by apply msqrtR.
-  - apply midR.
-  - apply mcosR.
-  - apply msinR.
-  - eapply ep_map; eauto. intros. by apply mcstR.
-  - eapply ep_map; eauto. intros. by apply mtruncateR.
-  - eapply ep_map2; eauto. intros ??. case is_leE=>//. auto.  
-  - eapply ep_map2; eauto. intros ??. case is_geE=>//. auto. 
-  - eapply ep_map2; eauto. intros ??. case is_ltE=>//. auto.
-  - eapply ep_map2; eauto. intros ??. case is_neE=>//. auto.
-  - by apply Eimpl_or.
-  - by apply Eimpl_and.
-  - eapply ep_bind=>[A Aa|]; eauto.
-    eapply ep_bind=>[B Bb|]; eauto.
+    eapply ep_bind=>[X Xx|]; eauto.
+    by apply mleE.
+  - eapply ep_map2; eauto=>??. case is_geE=>//. auto.  
+  - eapply ep_bind=>[F Ff|]; eauto. 
+    eapply ep_bind=>[X Xx|]; eauto.
+    by apply mgeE.
+  - eapply ep_map2; eauto=>??. case is_ltE=>//. auto.  
+  - eapply ep_bind=>[F Ff|]; eauto. 
+    eapply ep_bind=>[X Xx|]; eauto.
+    by apply mltE.
+  - eapply ep_map2; eauto=>??. case is_neE=>//. auto.  
+  - eapply ep_bind=>[F Ff|]; eauto. 
+    eapply ep_bind=>[X Xx|]; eauto.
+    constructor. by apply mneE.
+  - apply Eimpl_or'.
+    eapply Eimpl_impl. 2: apply IHtrel1. clear; auto. 
+    eapply Eimpl_impl. 2: apply IHtrel2. clear; auto.     
+  - apply Eimpl_or'.
+    eapply Eimpl_impl. 2: apply IHtrel1; eauto. clear; auto. 
+    eapply Eimpl_impl. 2: apply IHtrel2; eauto. clear; auto. 
+  - eapply Eimpl_and'.
+    apply IHtrel1; eassumption.
+    apply IHtrel2; eassumption.
+    auto.     
+  - eapply Eimpl_and'.
+    apply IHtrel1; eassumption.
+    apply IHtrel2; eassumption.
+    auto.     
+  - eapply ep_bind=>[A HA|]; eauto.
+    eapply ep_bind=>[B HB|]; eauto.
     eapply Eimpl_impl. 2: apply bisect2E.
     move=>K z Hz. cbn in *. eapply (K z); eauto.
-    clear A Aa B Bb. 
+    clear A HA B HB. 
     move=>A B. case_eq (is_lt A B)=>//=ab.
     apply Eimpl_forall=>z. 
     apply Eimpl_forall=>a. 
     apply Eimpl_forall=>b. 
-    apply Eimpl_forall=>Aa. 
-    apply Eimpl_forall=>Bb.
+    apply Eimpl_forall=>HA. 
+    apply Eimpl_forall=>HB.
     move: z. apply <-(Eimpl_forall (A:=R)).
-    apply IHtrel3. apply (M (DfromI2 Aa Bb ab)). 
-  - eapply ep_bind=>[A HA|]; eauto.
-    eapply ep_bind=>[B HB|]; eauto.
-    eapply Eimpl_impl. 2: apply bisectE.
-    move=>K z Hz. apply (K z). by eapply intervalE; eauto.
-    move=>X. apply Eimpl_forall=>z. apply Eimpl_forall=>Hz. by auto.
-  - eapply ep_bind=>[A Aa|]; eauto.  
-    eapply ep_bind=>[B Bb|]; eauto.
-    by apply mltE. 
-  - eapply ep_bind=>[A Aa|]; eauto.  
-    eapply ep_bind=>[B Bb|]; eauto.
-    constructor. by apply mneE. 
-  - apply Eimpl_or'.
-    eapply Eimpl_impl. 2: apply IHtrel1; eassumption. clear; auto. 
-    eapply Eimpl_impl. 2: apply IHtrel2; eassumption. clear; auto. 
-  - eapply Eimpl_and'.
-    apply IHtrel1; eassumption.
-    apply IHtrel2; eassumption.
-    auto. 
-  - eauto using Eimpl_impl. 
+    apply IHtrel3. apply (M (DfromI2 HA HB ab)). 
   - eapply ep_bind=>[A HA|]; eauto.
     eapply ep_bind=>[B HB|]; eauto.
     eapply Eimpl_impl. 2: apply bisectE.
     2: { move=>X. apply Eimpl_forall=>z. apply Eimpl_forall=>Hz. apply H2; eauto. } 
-    move=>K z Hz t Ht. apply K=>//. by eapply intervalE; eauto.
-  - auto.
+    move=>K z Hz. apply K=>//. by eapply intervalE; eauto.
+  - eapply ep_bind=>[A HA|]; eauto.
+    eapply ep_bind=>[B HB|]; eauto.
+    eapply Eimpl_impl. 2: apply bisectE.
+    2: { move=>X. apply Eimpl_forall=>z. apply Eimpl_forall=>Hz. apply H2; eauto. } 
+    move=>K z Hz t Ht. apply K=>//.
+    by eapply intervalE; eauto; apply mrangeR.
+  - auto. 
 Qed.
 
 (** correctness on parametric (closed) terms follows *)
-Lemma Correct: forall p S (u: Term S), parametric u -> cval (Sem' p u) (sem' u).
-Proof. intros p S u U. apply correct, U. Qed.
+Lemma Correct: forall p D C (u: Term D C), parametric u -> cval (Sem' p u) (sem' u).
+Proof. move=>*; by apply correct. Qed.
 
   
 (** small corollary, useful to obtain a tactic in tactic.v *)
-Lemma check p (b: Term BOOL):
+Lemma check p (b: Term ZER PROP):
   parametric b ->
   (let b := Sem' p b in
    match b with ret b => is_true b | err s => False end) ->
   sem' b.
 Proof.
-  move: (@Correct p BOOL)=>/= C B.
+  move: (@Correct p ZER PROP)=>/= C B.
   case C=>//. apply implE.
 Qed.
 
@@ -741,125 +750,47 @@ End Dynamic.
 
 
 (** ** notations for reified expressions *)
-(** mostly used for tests in tests.v for now 
-    sadly, trying to declare canonical structures of Ops0, Ops1, raises universe inconsistencies
- *)
+(** mostly used for tests in tests.v *)
 
-Definition expr X := @term X REAL.
-Definition fxpr X := @term X FUN.
-Definition bxpr X := @term X BOOL.
-Definition cxpr X := @term X PRED.
+Declare Scope term_scope.
+Bind Scope term_scope with term.
+Bind Scope term_scope with Term.
+Delimit Scope term_scope with term.
 
-Declare Scope expr_scope.
-Bind Scope expr_scope with expr.
-Delimit Scope expr_scope with expr.
-Definition e_add' X: expr X -> expr X -> expr X := e_add.
-Definition e_sub' X: expr X -> expr X -> expr X := e_sub.
-Definition e_mul' X: expr X -> expr X -> expr X := e_mul.
-Definition e_div' X: expr X -> expr X -> expr X := e_div.
-Infix "+" := e_add': expr_scope. 
-Infix "-" := e_sub': expr_scope.
-Infix "*" := e_mul': expr_scope.
-Infix "/" := e_div': expr_scope.
-Notation "0" := e_zer: expr_scope.
-Notation "1" := e_one: expr_scope.
-Definition fromQ' {X}: Q -> expr X := e_fromQ.
-Definition fromZ' {X}: Z -> expr X := e_fromZ.
-Definition sqrt' {X}: expr X -> expr X := e_sqrt.
-Definition cos' {X}: expr X -> expr X := e_cos.
-Definition sin' {X}: expr X -> expr X := e_sin.
-Definition abs' {X}: expr X -> expr X:= e_abs.
-Definition pi' {X}: expr X := e_pi.
+Notation TERM t := ((fun X => (t%term: @term X _ _)): Term _ _).
 
-Coercion cst' X: expr X -> fxpr X := f_cst.
-Declare Scope fxpr_scope.
-Bind Scope fxpr_scope with fxpr.
-Delimit Scope fxpr_scope with fxpr.
-Definition f_add' X: fxpr X -> fxpr X -> fxpr X := f_add.
-Definition f_sub' X: fxpr X -> fxpr X -> fxpr X := f_sub.
-Definition f_mul' X: fxpr X -> fxpr X -> fxpr X := f_mul.
-Definition f_div' X: fxpr X -> fxpr X -> fxpr X := f_div.
-Definition f_zer {X}: fxpr X := cst' 0. 
-Definition f_one {X}: fxpr X := cst' 1. 
-Infix "+" := f_add': fxpr_scope. 
-Infix "-" := f_sub': fxpr_scope.
-Infix "*" := f_mul': fxpr_scope.
-Infix "/" := f_div': fxpr_scope.
-Notation "0" := f_zer: fxpr_scope.
-Notation "1" := f_one: fxpr_scope.
+Notation id' := t_id.
+Notation integrate := t_integrate.
+Notation forall_models := t_forall_models.
+Notation forall_bisect := t_forall_bisect'.
+Notation cst := t_cst.
+Notation truncate := t_trunc.
+Notation truncate' := t_trunc'.
 
-Definition integrate' X: fxpr X -> expr X -> expr X -> expr X := e_integrate.
-Definition eval' X: fxpr X -> expr X -> expr X := e_eval.
-Definition id' {X}: fxpr X := f_id.
-Definition truncate' X: nat -> fxpr X -> fxpr X := f_trunc.
-Definition fsqrt X: fxpr X -> fxpr X := f_sqrt.
-Definition fcos X: fxpr X := f_cos.
-Definition fsin X: fxpr X := f_sin.
+Notation "'tlet' x := e 'in' g" := (t_let' e (fun x => g))
+    (at level 200, x binder, right associativity): term_scope.
 
-Declare Scope bxpr_scope.
-Bind Scope bxpr_scope with bxpr.
-Delimit Scope bxpr_scope with bxpr.
-Definition b_le' X: expr X -> expr X -> bxpr X := b_le.
-Definition b_ge' X: expr X -> expr X -> bxpr X := b_ge.
-Definition b_lt' X: expr X -> expr X -> bxpr X := b_lt.
-Definition b_gt' X e f: bxpr X := b_lt' f e.
-Definition b_conj' X: bxpr X -> bxpr X -> bxpr X := b_conj.
-Definition b_disj' X: bxpr X -> bxpr X -> bxpr X := b_disj.
-Infix "<=" := b_le': bxpr_scope. 
-Infix "<" := b_lt': bxpr_scope. 
-Infix ">=" := b_ge': bxpr_scope. 
-Infix ">" := b_gt': bxpr_scope. 
-Infix "/\" := b_conj': bxpr_scope. 
-Infix "\/" := b_disj': bxpr_scope.
-
-Declare Scope cxpr_scope.
-Bind Scope cxpr_scope with cxpr.
-Delimit Scope cxpr_scope with cxpr.
-Definition c_lt' X: fxpr X -> fxpr X -> cxpr X := c_lt.
-Definition c_ne' X: fxpr X -> fxpr X -> cxpr X := c_ne.
-Definition c_conj' X: cxpr X -> cxpr X -> cxpr X := c_conj.
-Definition c_disj' X: cxpr X -> cxpr X -> cxpr X := c_disj.
-Coercion c_cst' X: bxpr X -> cxpr X := c_cst.
-Infix "<" := c_lt': cxpr_scope. 
-Infix "<>" := c_ne': cxpr_scope. 
-Infix "/\" := c_conj': cxpr_scope. 
-Infix "\/" := c_disj': cxpr_scope.
-
-Definition b_forall_models' {X}: expr X -> expr X -> cxpr X -> bxpr X :=
-  b_forall_models.
-Definition b_forall_bisect' {X} (a b: expr X) (f: expr X -> bxpr X): bxpr X :=
-  b_forall_bisect a b (fun x => f (t_var x)).
-Definition c_forall_bisect' {X} (a b: expr X) (f: expr X -> cxpr X): cxpr X :=
-  c_forall_bisect a b (fun x => f (t_var x)).
-Arguments b_forall_bisect' {_} (_ _)%expr _%bxpr.
-Arguments c_forall_bisect' {_} (_ _)%expr _%cxpr.
-
-Notation "'let_e' x := e 'in' g" := (let' (e%expr: expr _) (fun (x: expr _) => (g%expr: expr _))) (at level 200, x binder, right associativity): expr_scope.
-Notation "'let_e' x := e 'in' g" := (let' (e%expr: expr _) (fun (x: expr _) => (g%fxpr: fxpr _))) (at level 200, x binder, right associativity): fxpr_scope.
-Notation "'let_e' x := e 'in' g" := (let' (e%expr: expr _) (fun (x: expr _) => (g%bxpr: bxpr _))) (at level 200, x binder, right associativity): bxpr_scope.
-Notation "'let_e' x := e 'in' g" := (let' (e%expr: expr _) (fun (x: expr _) => (g%cxpr: cxpr _))) (at level 200, x binder, right associativity): cxpr_scope.
-Notation "'let_f' x := e 'in' g" := (let' (e%fxpr: fxpr _) (fun (x: fxpr _) => (g%expr: expr _))) (at level 200, x binder, right associativity): expr_scope.
-Notation "'let_f' x := e 'in' g" := (let' (e%fxpr: fxpr _) (fun (x: fxpr _) => (g%fxpr: fxpr _))) (at level 200, x binder, right associativity): fxpr_scope.
-Notation "'let_f' x := e 'in' g" := (let' (e%fxpr: fxpr _) (fun (x: fxpr _) => (g%bxpr: bxpr _))) (at level 200, x binder, right associativity): bxpr_scope.
-Notation "'let_f' x := e 'in' g" := (let' (e%fxpr: fxpr _) (fun (x: fxpr _) => (g%cxpr: cxpr _))) (at level 200, x binder, right associativity): cxpr_scope.
-
-Notation EXPR t := ((fun X => (t%expr: expr X)): Term REAL).
-Notation FXPR t := ((fun X => (t%fxpr: fxpr X)): Term FUN).
-Notation BXPR t := ((fun X => (t%bxpr: bxpr X)): Term BOOL).
-Notation CXPR t := ((fun X => (t%cxpr: cxpr X)): Term PRED).
+Infix "<=" := t_le: term_scope. 
+Infix "<" := t_lt: term_scope. 
+Infix ">=" := t_ge: term_scope. 
+Notation "a > b" := (t_lt b a): term_scope. 
+Infix "<>" := t_ne: term_scope. 
+Infix "/\" := t_conj: term_scope. 
+Infix "\/" := t_disj: term_scope.
 
 (*
-Check EXPR (1+e_pi).
-Check EXPR (1+integrate' id' 0 1).
-Check FXPR (id'/id').
-Check EXPR (1+integrate' (id' / fsqrt id') 0 (fromQ' 3.3)).
-Check EXPR (1+integrate' (id' / (fsqrt id' + fromZ' 3)) 0 (fromQ' 3.3)).
-Check EXPR (1+integrate' (id' / (fsqrt id' + fromZ' 3)) 0 (fromQ' 3.3)).
-Check EXPR (let_e x := 1+e_pi in x + x).
-Check EXPR (let_e x := 1+e_pi in x + let_e y := x*x in sqrt' (y+y)).
-Check FXPR (let_e x := 1+e_pi in id' + x).
-Check FXPR (let_f f := 1-id' in id' * id').
-Check BXPR (1 <= 0 \/ cos' pi' < 1 /\ cos' 0 >= 1).
-Check BXPR (b_forall_bisect' 0 1 (fun c => integrate' (id'+c) 0 1 <= c+1/fromZ' 2) ).
-Check BXPR (b_forall_models' 0 1 (id' < 0 /\ 1 <> fsqrt id')).
+Fail Check Dynamic.check _ _ (TERM (1<pi)).
+Check TERM (1+pi).
+Check TERM (1+integrate id' 0 1).
+Check TERM (id'/id').
+Check TERM (1+integrate (id' / sqrt id') 0 (fromQ 3.3)).
+Check TERM (1+integrate (id' / (sqrt id' + fromZ 3)) 0 (fromQ 3.3)).
+Check TERM (tlet x := 1+pi in x + x).
+Check TERM (tlet x := 1+pi in x + tlet y := x*x in sqrt (y+y)).
+Check TERM (tlet x := 1+pi in id' + x).
+Check TERM (tlet f := 1-id' in id' * id').
+Check TERM (tlet f := 1-id' in id' *[4] id').
+Check TERM (1 <= 0 \/ cos pi < 1 /\ cos 0 >= 1).
+Check TERM (forall_bisect 0 1 (fun c => integrate (id'+cst c) 0 1 <= c+1/fromZ 2) ).
+Check TERM (truncate 4 (cos id')).
 *) 
